Complete proofs in Pact.v

src/Eval.v
@@ -1,7 +1,9 @@
 Require Import
   Coq.Unicode.Utf8
   Coq.Lists.List
-  Coq.Logic.Classical
+  Coq.Relations.Relation_Definitions
+  Coq.Classes.RelationClasses
+  Coq.Classes.Morphisms
   Ty
   Exp
   Sub
@@ -93,9 +95,54 @@ Inductive Step : ∀ {Γ τ}, Exp Γ τ → Exp Γ τ → Prop :=
 
 Derive Signature for Step.
 
+Inductive multi {X : Type} (R : relation X) : relation X :=
+  | multi_refl (x : X) : multi R x x
+  | multi_step (x y z : X) :
+      R x y → multi R y z → multi R x z.
+
+Derive Signature for multi.
+
+Theorem multi_R (X : Type) (R : relation X) (x y : X) :
+  R x y → multi R x y.
+Proof.
+  intros.
+  eapply multi_step; eauto.
+  now constructor.
+Qed.
+
+Theorem multi_trans (X : Type) (R : relation X) (x y z : X) :
+  multi R x y →
+  multi R y z →
+  multi R x z.
+Proof.
+  intros.
+  induction H; auto.
+  now eapply multi_step; eauto.
+Qed.
+
+#[export]
+Program Instance multi_PreOrder (X : Type) (R : relation X) :
+  PreOrder (multi R).
+Next Obligation. now constructor. Qed.
+Next Obligation. now eapply multi_trans; eauto. Qed.
+
+#[export]
+Program Instance Step_respects {Γ τ} :
+  Proper (Step --> Step ==> impl) (multi (Step (Γ:=Γ) (τ:=τ))).
+Next Obligation.
+  econstructor; eauto.
+  generalize dependent y0.
+  generalize dependent y.
+  induction H1; intros; eauto.
+  - now repeat econstructor; eauto.
+  - unfold flip in *.
+    now econstructor; eauto.
+Qed.
+
 End Eval.
 
 Notation " t '--->' t' " := (Step t t') (at level 40).
+Notation " t '--->*' t' " := (multi Step t t') (at level 40).
 
 Class HostLang (A : Type) : Type := {
   has_host_exprs_sem :> HostExprsSem A;
@@ -149,6 +196,193 @@ Proof.
     f_equal; simpl.
     simp SubSem.
     now rewrite SubSem_idSub.
+Qed.
+
+Lemma If_loop_true {Γ τ} b {x : Exp Γ τ} {y : Exp Γ τ} :
+  ¬ (If b x y = x).
+Proof.
+  induction x; intro; inv H.
+  now eapply IHx2; eauto.
+Qed.
+
+Lemma If_loop_false {Γ τ} b {x : Exp Γ τ} {y : Exp Γ τ} :
+  ¬ (If b x y = y).
+Proof.
+  induction y; intro; inv H.
+  now eapply IHy3; eauto.
+Qed.
+
+Lemma Seq_loop {Γ τ ty} {x : Exp Γ ty} {y : Exp Γ τ} :
+  ¬ (Seq x y = y).
+Proof.
+  induction y; intro; inv H.
+  now eapply IHy2; eauto.
+Qed.
+
+Lemma App_Lam_loop {Γ τ ty} {v : Exp Γ ty} {e : Exp (ty :: Γ) τ} :
+  ¬ (SubExp {||v||} e = APP (LAM e) v).
+Proof.
+  dependent induction e; repeat intro; inv H.
+  - dependent induction v0; simp consSub in *.
+    + simp SubVar in H1.
+      now induction v; inv H1; intuition.
+    + simp SubVar in H1.
+      rewrite SubVar_idSub in H1.
+      now induction v0; inv H1; intuition.
+  - admit.
+Admitted.
+
+(* A term never reduces to itself. *)
+#[export]
+Program Instance Step_Irreflexive {Γ τ} :
+  Irreflexive (Step (Γ:=Γ) (τ:=τ)).
+Next Obligation.
+  dependent induction x; try solve [ now inv H ].
+  - inv H.
+    + now apply Reduce_irr in H4.
+  - inv H.
+    + now eapply If_loop_true; eauto.
+    + now eapply If_loop_false; eauto.
+    + now firstorder.
+  - inv H.
+    now eapply Seq_loop; eauto.
+  - inv H.
+    + now eapply CallHost_irr; eauto.
+    + now eapply App_Lam_loop; eauto.
+    + now eapply IHx1; eauto.
+    + now eapply IHx2; eauto.
+Qed.
+
+#[export]
+Program Instance RenExp_Step {Γ Γ' τ} (σ : Ren Γ' Γ) :
+  Proper (Step (Γ:=Γ) (τ:=τ) ==> Step) (RenExp σ).
+Next Obligation.
+  intros.
+  induction H; simpl;
+  try solve [ now constructor; intuition idtac
+            | now constructor; intuition; apply RenExp_ValueP ].
+  - now apply Reduce_preserves_renaming.
+  - now apply CallHost_preserves_renaming.
+  - rewrite <- SubExp_ScR.
+    simp ScR.
+    rewrite <- RcS_idSub.
+    pose proof (SubExp_RcS (Keep σ) (Push (RenExp σ v) idSub) e).
+    simp RcS in H.
+    rewrite H.
+    constructor.
+    now apply RenExp_ValueP.
+Qed.
+
+#[export]
+Program Instance SubExp_Step {Γ Γ' τ} (σ : Sub Γ' Γ) :
+  Proper (Step (Γ:=Γ) (τ:=τ) ==> Step) (SubExp σ).
+Next Obligation.
+  intros.
+  induction H; simpl;
+  try solve [ now constructor; intuition idtac
+            | now constructor; intuition; apply SubExp_ValueP ].
+  - now apply Reduce_preserves_substitution.
+  - now apply CallHost_preserves_substitution.
+  - rewrite <- SubExp_ScS.
+    simpl ScS.
+    rewrite ScS_idSub_left.
+    pose proof (SubExp_ScS (Keepₛ σ) (Push (SubExp σ v) idSub) e).
+    simpl in H.
+    simp SubVar in H.
+    unfold Dropₛ in H.
+    rewrite ScS_ScR in H.
+    rewrite RcS_skip1 in H.
+    rewrite ScS_idSub_right in H.
+    rewrite H.
+    constructor.
+    now apply SubExp_ValueP.
+Qed.
+
+Corollary Step_productive {Γ τ} {x x' : Exp Γ τ} : x ---> x' → x ≠ x'.
+Proof.
+  repeat intro; subst.
+  now eapply Step_Irreflexive; eauto.
+Qed.
+
+Import ListNotations.
+
+Theorem strong_progress {τ} (e : Exp [] τ) :
+  ValueP e + { e' | e ---> e' }.
+Proof.
+  dependent induction e.
+  - destruct τ;
+    right; now exists (projT1 (Reduce h)); constructor.
+  - now left; constructor.
+  - now left; constructor.
+  - now left; constructor.
+  - now left; constructor.
+  - now left; constructor.
+  - right.
+    destruct (IHe1 _ _ _ eq_refl JMeq_refl JMeq_refl JMeq_refl); reduce.
+    + inv v.
+      * now exists e2; constructor.
+      * now exists e3; constructor.
+    + reduce.
+      now exists (If x e2 e3); constructor.
+  - destruct (IHe1 _ _ _ eq_refl JMeq_refl JMeq_refl JMeq_refl); reduce.
+    + destruct (IHe2 _ _ _ eq_refl JMeq_refl JMeq_refl JMeq_refl); reduce.
+      * left.
+        now constructor.
+      * right; reduce.
+        now exists (Pair e1 x); constructor.
+    + destruct (IHe2 _ _ _ eq_refl JMeq_refl JMeq_refl JMeq_refl); reduce.
+      * right; reduce.
+        now exists (Pair x e2); constructor.
+      * right; reduce.
+        now exists (Pair x e2); constructor.
+  - destruct (IHe _ _ _ eq_refl JMeq_refl JMeq_refl JMeq_refl); reduce.
+    + right.
+      inv v; reduce.
+      * now exists x; constructor.
+    + right; reduce.
+      now exists (Fst x); constructor.
+  - destruct (IHe _ _ _ eq_refl JMeq_refl JMeq_refl JMeq_refl); reduce.
+    + right.
+      inv v.
+      * now exists y; constructor.
+    + right; reduce.
+      now exists (Snd x); constructor.
+  - now left; constructor.
+  - destruct (IHe1 _ _ _ eq_refl JMeq_refl JMeq_refl JMeq_refl); clear IHe1.
+    + destruct (IHe2 _ _ _ eq_refl JMeq_refl JMeq_refl JMeq_refl); clear IHe2.
+      * now left; constructor.
+      * right; reduce.
+        now exists (Cons e1 x); constructor.
+    + destruct (IHe2 _ _ _ eq_refl JMeq_refl JMeq_refl JMeq_refl); clear IHe2.
+      * right; reduce.
+        now exists (Cons x e2); constructor.
+      * right; reduce.
+        now exists (Cons x0 e2); constructor.
+  - right.
+    now exists e2; constructor.
+  - now inversion v.
+  - left.
+    now constructor.
+  - right.
+    destruct (IHe1 _ _ _ eq_refl JMeq_refl JMeq_refl JMeq_refl); clear IHe1.
+    + destruct (IHe2 _ _ _ eq_refl JMeq_refl JMeq_refl JMeq_refl); clear IHe2.
+      * dependent elimination e1; inv v.
+        ** now exists (CallHost h1 e2 v0); constructor.
+        ** exists (SubExp {|| e2 ||} e11).
+           now constructor.
+      * dependent elimination e1; inv v.
+        ** exists (APP (HostedFun h1) x); constructor; auto.
+           now constructor.
+        ** exists (APP (LAM e11) x).
+           constructor; auto.
+           now constructor.
+    + reduce.
+      destruct (IHe2 _ _ _ eq_refl JMeq_refl JMeq_refl JMeq_refl); clear IHe2.
+      * exists (APP x e2).
+        now constructor.
+      * reduce.
+        exists (APP x e2).
+        now constructor.
 Qed.
 
 End Sound.
