src/Norm.v
@@ -1,9 +1,10 @@
 Require Import
   Coq.Unicode.Utf8
   Coq.Program.Program
+  Coq.Lists.List
   Coq.Relations.Relation_Definitions
   Coq.Classes.CRelationClasses
-  Coq.Lists.List
+  Coq.Classes.Morphisms
   Ty
   Exp
   Sub
@@ -49,66 +50,6 @@ Ltac normality :=
         now exists Y
   end.
 
-Lemma If_loop_true {Γ τ} b {x : Exp Γ τ} {y : Exp Γ τ} :
-  ¬ (If b x y = x).
-Proof.
-  induction x; intro; inv H.
-  now eapply IHx2; eauto.
-Qed.
-
-Lemma If_loop_false {Γ τ} b {x : Exp Γ τ} {y : Exp Γ τ} :
-  ¬ (If b x y = y).
-Proof.
-  induction y; intro; inv H.
-  now eapply IHy3; eauto.
-Qed.
-
-Lemma Seq_loop {Γ τ ty} {x : Exp Γ ty} {y : Exp Γ τ} :
-  ¬ (Seq x y = y).
-Proof.
-  induction y; intro; inv H.
-  now eapply IHy2; eauto.
-Qed.
-
-Lemma App_Lam_loop {Γ τ ty} {v : Exp Γ ty} {e : Exp (ty :: Γ) τ} :
-  ¬ (SubExp {||v||} e = APP (LAM e) v).
-Proof.
-  dependent induction e; repeat intro; inv H.
-  - dependent induction v0; simp consSub in *.
-    + simp SubVar in H1.
-      now induction v; inv H1; intuition.
-    + simp SubVar in H1.
-      rewrite SubVar_idSub in H1.
-      now induction v0; inv H1; intuition.
-  - admit.
-Admitted.
-
-(* A term never reduces to itself. *)
-Theorem Step_irr {Γ τ} {x : Exp Γ τ} : ¬ (x ---> x).
-Proof.
-  intro.
-  dependent induction x; try solve [ now inv H ].
-  - inv H.
-    + now apply Reduce_irr in H4.
-  - inv H.
-    + now eapply If_loop_true; eauto.
-    + now eapply If_loop_false; eauto.
-    + now firstorder.
-  - inv H.
-    now eapply Seq_loop; eauto.
-  - inv H.
-    + now eapply CallHost_irr; eauto.
-    + now eapply App_Lam_loop; eauto.
-    + now eapply IHx1; eauto.
-    + now eapply IHx2; eauto.
-Qed.
-
-Corollary Step_productive {Γ τ} {x x' : Exp Γ τ} : x ---> x' → x ≠ x'.
-Proof.
-  repeat intro; subst.
-  now eapply Step_irr; eauto.
-Qed.
-
 Ltac invert_step :=
   try lazymatch goal with
   | [ H : _ ---> _ |- _ ] => now inv H
@@ -132,85 +73,6 @@ Proof.
   - now f_equal; apply ValueP_irrelevance.
 Qed.
 
-Theorem strong_progress {τ} (e : Exp [] τ) :
-  ValueP e + { e' | e ---> e' }.
-Proof.
-  dependent induction e.
-  - destruct τ;
-    right; now exists (projT1 (Reduce h)); constructor.
-  - now left; constructor.
-  - now left; constructor.
-  - now left; constructor.
-  - now left; constructor.
-  - now left; constructor.
-  - right.
-    destruct (IHe1 _ _ _ eq_refl JMeq_refl JMeq_refl JMeq_refl); reduce.
-    + inv v.
-      * now exists e2; constructor.
-      * now exists e3; constructor.
-    + reduce.
-      now exists (If x e2 e3); constructor.
-  - destruct (IHe1 _ _ _ eq_refl JMeq_refl JMeq_refl JMeq_refl); reduce.
-    + destruct (IHe2 _ _ _ eq_refl JMeq_refl JMeq_refl JMeq_refl); reduce.
-      * left.
-        now constructor.
-      * right; reduce.
-        now exists (Pair e1 x); constructor.
-    + destruct (IHe2 _ _ _ eq_refl JMeq_refl JMeq_refl JMeq_refl); reduce.
-      * right; reduce.
-        now exists (Pair x e2); constructor.
-      * right; reduce.
-        now exists (Pair x e2); constructor.
-  - destruct (IHe _ _ _ eq_refl JMeq_refl JMeq_refl JMeq_refl); reduce.
-    + right.
-      inv v; reduce.
-      * now exists x; constructor.
-    + right; reduce.
-      now exists (Fst x); constructor.
-  - destruct (IHe _ _ _ eq_refl JMeq_refl JMeq_refl JMeq_refl); reduce.
-    + right.
-      inv v.
-      * now exists y; constructor.
-    + right; reduce.
-      now exists (Snd x); constructor.
-  - now left; constructor.
-  - destruct (IHe1 _ _ _ eq_refl JMeq_refl JMeq_refl JMeq_refl); clear IHe1.
-    + destruct (IHe2 _ _ _ eq_refl JMeq_refl JMeq_refl JMeq_refl); clear IHe2.
-      * now left; constructor.
-      * right; reduce.
-        now exists (Cons e1 x); constructor.
-    + destruct (IHe2 _ _ _ eq_refl JMeq_refl JMeq_refl JMeq_refl); clear IHe2.
-      * right; reduce.
-        now exists (Cons x e2); constructor.
-      * right; reduce.
-        now exists (Cons x0 e2); constructor.
-  - right.
-    now exists e2; constructor.
-  - now inversion v.
-  - left.
-    now constructor.
-  - right.
-    destruct (IHe1 _ _ _ eq_refl JMeq_refl JMeq_refl JMeq_refl); clear IHe1.
-    + destruct (IHe2 _ _ _ eq_refl JMeq_refl JMeq_refl JMeq_refl); clear IHe2.
-      * dependent elimination e1; inv v.
-        ** now exists (CallHost h1 e2 v0); constructor.
-        ** exists (SubExp {|| e2 ||} e11).
-           now constructor.
-      * dependent elimination e1; inv v.
-        ** exists (APP (HostedFun h1) x); constructor; auto.
-           now constructor.
-        ** exists (APP (LAM e11) x).
-           constructor; auto.
-           now constructor.
-    + reduce.
-      destruct (IHe2 _ _ _ eq_refl JMeq_refl JMeq_refl JMeq_refl); clear IHe2.
-      * exists (APP x e2).
-        now constructor.
-      * reduce.
-        exists (APP x e2).
-        now constructor.
-Qed.
-
 Corollary nf_is_value {τ} (v : Exp [] τ) :
   normal_form Step v → ValueP v.
 Proof.
@@ -227,33 +89,6 @@ Proof.
   split.
   - now apply nf_is_value.
   - now apply value_is_nf.
-Qed.
-
-Inductive multi {X : Type} (R : relation X) : relation X :=
-  | multi_refl : ∀ (x : X), multi R x x
-  | multi_step : ∀ (x y z : X),
-      R x y →
-      multi R y z →
-      multi R x z.
-
-Notation " t '--->*' t' " := (multi Step t t') (at level 40).
-
-Theorem multi_R : ∀ (X : Type) (R : relation X) (x y : X),
-  R x y → (multi R) x y.
-Proof.
-  intros.
-  eapply multi_step; eauto.
-  now constructor.
-Qed.
-
-Theorem multi_trans : ∀ (X : Type) (R : relation X) (x y z : X),
-  multi R x y →
-  multi R y z →
-  multi R x z.
-Proof.
-  intros.
-  induction H; auto.
-  now eapply multi_step; eauto.
 Qed.
 
 Definition halts {Γ τ} (e : Exp Γ τ) : Prop :=
@@ -411,89 +246,6 @@ Lemma msubst_R : ∀ Γ (env : ExpEnv Γ) τ (t : Exp Γ τ),
 Proof.
 *)
 
-Lemma RenExp_ValueP {Γ Γ' τ} {v : Exp Γ τ} (σ : Ren Γ' Γ) :
-  ValueP v → ValueP (RenExp σ v).
-Proof.
-  intros.
-  now induction X; simpl; intros; try constructor.
-Qed.
-
-Lemma SubExp_ValueP {Γ Γ' τ} {v : Exp Γ τ} (σ : Sub Γ' Γ) :
-  ValueP v → ValueP (SubExp σ v).
-Proof.
-  intros.
-  now induction X; simpl; intros; try constructor.
-Qed.
-
-Lemma RenExp_Step {Γ Γ' τ} {e e' : Exp Γ τ} (σ : Ren Γ' Γ) :
-  e ---> e' → RenExp σ e ---> RenExp σ e'.
-Proof.
-  intros.
-  induction e; simpl; invert_step.
-  - destruct τ;
-    inv H; now apply Reduce_preserves_renaming.
-  - now inv H; constructor; intuition.
-  - inv H; simpl;
-    constructor; intuition;
-    now apply RenExp_ValueP.
-  - inv H; constructor; intuition.
-    + now apply RenExp_ValueP.
-    + now apply RenExp_ValueP.
-  - inv H; constructor; intuition.
-    + now apply RenExp_ValueP.
-    + now apply RenExp_ValueP.
-  - inv H; constructor; intuition;
-    now apply RenExp_ValueP.
-  - now inv H; simpl; try constructor; intuition.
-  - inv H; simpl; try constructor; intuition.
-    + rewrite <- SubExp_ScR.
-      simp ScR.
-      rewrite <- RcS_idSub.
-      pose proof (SubExp_RcS (Keep σ) (Push (RenExp σ e2) idSub) e0).
-      simp RcS in H.
-      rewrite H.
-      constructor.
-      now apply RenExp_ValueP.
-    + now apply RenExp_ValueP.
-Qed.
-
-Lemma SubExp_Step {Γ Γ' τ} {e e' : Exp Γ τ} (σ : Sub Γ' Γ) :
-  e ---> e' → SubExp σ e ---> SubExp σ e'.
-Proof.
-  intros.
-  induction e; simpl; invert_step.
-  - destruct τ;
-    inv H; now apply Reduce_preserves_substitution.
-  - now inv H; constructor; intuition.
-  - inv H; simpl;
-    constructor; intuition;
-    now apply SubExp_ValueP.
-  - inv H; constructor; intuition.
-    + now apply SubExp_ValueP.
-    + now apply SubExp_ValueP.
-  - inv H; constructor; intuition.
-    + now apply SubExp_ValueP.
-    + now apply SubExp_ValueP.
-  - inv H; constructor; intuition;
-    now apply SubExp_ValueP.
-  - now inv H; simpl; try constructor; intuition.
-  - inv H; simpl; try constructor; intuition.
-    + rewrite <- SubExp_ScS.
-      simpl ScS.
-      rewrite ScS_idSub_left.
-      pose proof (SubExp_ScS (Keepₛ σ) (Push (SubExp σ e2) idSub) e0).
-      simpl in H.
-      simp SubVar in H.
-      unfold Dropₛ in H.
-      rewrite ScS_ScR in H.
-      rewrite RcS_skip1 in H.
-      rewrite ScS_idSub_right in H.
-      rewrite H.
-      constructor.
-      now apply SubExp_ValueP.
-    + now apply SubExp_ValueP.
-Qed.
-
 (*
 Equations RenExp_Step {Γ Γ' τ} {e : Exp Γ τ} {σ : Ren Γ' Γ} {e'}
           (S : RenExp σ e ---> e') :
@@ -644,5 +396,3 @@ strongNorm t = coe (SN & Tm-idₛ t) (SN*-SN (fth t idₛᴾ))
 *)
 
 End Norm.
-
-Notation " t '--->*' t' " := (multi Step t t') (at level 40).
