src/Ren.v
@@ -31,9 +31,9 @@ Fixpoint idRen {Γ} : Ren Γ Γ :=
 Lemma Keep_idRen {Γ τ} : Keep (τ:=τ) (@idRen Γ) = idRen.
 Proof. now induction Γ. Qed.
 
-Equations DropAll Γ : Ren Γ [] :=
-  DropAll []        := NoRen;
-  DropAll (x :: xs) := Drop (DropAll xs).
+Equations DropAll {Γ} : Ren Γ [] :=
+  DropAll (Γ:=[])      := NoRen;
+  DropAll (Γ:=_ :: xs) := Drop (DropAll (Γ:=xs)).
 
 Corollary NoRen_idRen : NoRen = idRen.
 Proof. reflexivity. Qed.
